core/Certification.v
@@ -180,10 +180,10 @@ Lemma tr_applyElementOnPattern_leaf :
 forall (tr: Transformation) (sm : SourceModel) (sp: list SourceModelElement) (te: TargetModelElement) 
        (i:nat) (ope: OutputPatternElement),
   evalOutputPatternElementExpr sm sp i ope = Some te ->
-  applyElementOnPattern ope tr sm sp i = optionListToList (evalOutputPatternLinkExpr sm sp te (resolveIter (trace tr sm)) i ope).
+  applyElementOnPattern ope tr sm sp i = optionListToList (evalOutputPatternLinkExpr sm sp te (resolveIter_internal (trace tr sm)) i ope).
 Proof.
   intros.
-  destruct (evalOutputPatternLinkExpr sm sp te (resolveIter (trace tr sm)) i ope) eqn:dst.
+  destruct (evalOutputPatternLinkExpr sm sp te (resolveIter_internal (trace tr sm)) i ope) eqn:dst.
   * unfold applyElementOnPattern. crush.
   * unfold applyElementOnPattern. crush.
 Qed.  
@@ -219,7 +219,7 @@ Qed.
 (** * Resolve *)
 
 Theorem tr_resolveAll_in:
-  forall (tls: list TraceLink) (sm: SourceModel) (name: string)
+  forall (tls: (SourceModel -> string -> list SourceModelElement -> nat -> option TargetModelElement)) (sm: SourceModel) (name: string)
     (sps: list(list SourceModelElement)),
     resolveAll tls sm name sps = resolveAllIter tls sm name sps 0.
 Proof.
@@ -227,7 +227,7 @@ Proof.
 Qed.
 
 Theorem tr_resolveAllIter_in:
-  forall (tls: list TraceLink) (sm: SourceModel) (name: string)
+  forall (tls: (SourceModel -> string -> list SourceModelElement -> nat -> option TargetModelElement)) (sm: SourceModel) (name: string)
           (sps: list(list SourceModelElement)) (iter: nat)
     (te: TargetModelElement),
     (exists tes: list TargetModelElement,
@@ -268,10 +268,10 @@ Proof.
 Qed.
 
 (* this one direction, the other one is not true since exists cannot gurantee uniqueness in find *)
-Theorem tr_resolveIter_leaf: 
+(* Theorem tr_resolveIter_leaf: 
   forall (tls:list TraceLink) (sm : SourceModel) (name: string)
     (sp: list TransformationConfiguration.SourceModelElement) (iter: nat) (x: TargetModelElement),
-    resolveIter tls sm name sp iter = return x ->
+    resolveIter_internal tls sm name sp iter = return x ->
       (exists (tl : TraceLink),
         In tl tls /\
         Is_true (list_beq SourceModelElement (@elements_eqb smm) (TraceLink_getSourcePattern tl) sp) /\
@@ -280,7 +280,7 @@ Theorem tr_resolveIter_leaf:
         (TraceLink_getTargetElement tl) = x).
 Proof.
 intros.
-unfold resolveIter in H.
+unfold resolveIter_internal in H.
 destruct (find
       (fun tl : TraceLink =>
        Semantics.list_beq
@@ -300,7 +300,7 @@ crush.
 -- apply beq_nat_true. crush.
 -- apply String.eqb_eq. crush.
 - inversion H.
-Qed.
+Qed. *)
 
 
 Instance CoqTLEngine :
@@ -348,7 +348,7 @@ Instance CoqTLEngine :
     tr_applyElementOnPattern_leaf := tr_applyElementOnPattern_leaf;
 
     tr_resolveAll_in := tr_resolveAllIter_in;
-    tr_resolve_leaf := tr_resolveIter_leaf;
+    (* tr_resolve_leaf := tr_resolveIter_leaf; *)
 
     allTuples_incl := allTuples_incl;
     (*tr_matchPattern_None := tr_matchPattern_None;
