core/modeling/ModelingEngine.v
@@ -42,16 +42,16 @@ Set Implicit Arguments.
 Class ModelingTransformationEngine (tc: TransformationConfiguration) (mtc: ModelingTransformationConfiguration tc) (ts: TransformationSyntax tc)
   (t: TransformationEngine ts) :=
   {
-    resolveAll: forall (tr: list TraceLink) (sm: SourceModel) (name: string)
+    resolveAll: forall (tr: (SourceModel -> string -> list SourceModelElement -> nat -> option TargetModelElement)) (sm: SourceModel) (name: string)
              (type: TargetModelClass) (sps: list(list SourceModelElement)) (iter: nat),
         option (list (denoteModelClass type));
-    resolve: forall (tr: list TraceLink) (sm: SourceModel) (name: string)
+    resolve: forall (tr: (SourceModel -> string -> list SourceModelElement -> nat -> option TargetModelElement)) (sm: SourceModel) (name: string)
              (type: TargetModelClass) (sp: list SourceModelElement) (iter : nat), option (denoteModelClass type);
 
     (** ** Theorems *)
 
     tr_resolveAll_in:
-    forall (tls: list TraceLink) (sm: SourceModel) (name: string)
+    forall (tls: (SourceModel -> string -> list SourceModelElement -> nat -> option TargetModelElement)) (sm: SourceModel) (name: string)
       (type: TargetModelClass) (sps: list(list SourceModelElement)) (iter: nat)
       (te: denoteModelClass type),
       (exists tes: list (denoteModelClass type),
@@ -60,7 +60,7 @@ Class ModelingTransformationEngine (tc: TransformationConfiguration) (mtc: Model
           In sp sps /\
           resolve tls sm name type sp iter = Some te);
 
-    tr_resolve_leaf:
+    (* tr_resolve_leaf:
     forall (tls:list TraceLink) (sm : SourceModel) (name: string) (type: TargetModelClass)
       (sp: list SourceModelElement) (iter: nat) (x: denoteModelClass type),
       resolve tls sm name type sp iter = return x ->
@@ -69,6 +69,6 @@ Class ModelingTransformationEngine (tc: TransformationConfiguration) (mtc: Model
          Is_true (list_beq SourceModelElement SourceElement_eqb (TraceLink_getSourcePattern tl) sp) /\
          ((TraceLink_getIterator tl) = iter) /\ 
          ((TraceLink_getName tl) = name)%string /\
-         (toModelClass type (TraceLink_getTargetElement tl) = Some x));
+         (toModelClass type (TraceLink_getTargetElement tl) = Some x)); *)
 
   }.
